wip

crypto_hst/Hacl.Box.fst
@@ -2,8 +2,9 @@ module Hacl.Box
 
 open FStar.Buffer
 open FStar.HST
-open Hacl.Constants
 
+open Hacl.Constants
+open Hacl.SecretBox
 
 (* Module abbreviations *)
 module HS  = FStar.HyperStack
@@ -11,6 +12,7 @@ module B   = FStar.Buffer
 module U8  = FStar.UInt8
 module U32 = FStar.UInt32
 module U64 = FStar.UInt64
+
 
 
 val crypto_box_easy:
@@ -23,6 +25,14 @@ val crypto_box_easy:
   Stack u32
     (requires (fun h -> live h c /\ live h m /\ live h n /\ live h pk /\ live h sk))
     (ensures  (fun h0 z h1 -> modifies_1 c h0 h1 /\ live h1 c))
+let crypto_box_easy c m mlen n pk sk =
+  push_frame();
+  let key = create (Hacl.Cast.uint8_to_sint8 0uy) 32ul in
+  (* Compute shared key *)
+  Hacl.EC.Curve25519.exp key pk sk;
+  let z = crypto_secretbox_easy c m mlen n key in
+  pop_frame();
+  z
 
 
 val crypto_box_open_easy:
@@ -35,6 +45,14 @@ val crypto_box_open_easy:
   Stack u32
     (requires (fun h -> live h c /\ live h m /\ live h n /\ live h pk /\ live h sk))
     (ensures  (fun h0 z h1 -> modifies_1 c h0 h1 /\ live h1 c))
+let crypto_box_open_easy m c mlen n pk sk =
+  push_frame();
+  let key = create (Hacl.Cast.uint8_to_sint8 0uy) 32ul in
+  (* Compute shared key *)
+  Hacl.EC.Curve25519.exp key pk sk;
+  let z = crypto_secretbox_open_easy m c mlen n key in
+  pop_frame();
+  z
 
 
 val crypto_box_detached:
@@ -48,9 +66,17 @@ val crypto_box_detached:
   Stack u32
     (requires (fun h -> live h c /\ live h m /\ live h n /\ live h pk /\ live h sk))
     (ensures  (fun h0 z h1 -> modifies_1 c h0 h1 /\ live h1 c))
+let crypto_box_detached c mac m mlen n pk sk =
+  push_frame();
+  let key = create (Hacl.Cast.uint8_to_sint8 0uy) 32ul in
+  (* Compute shared key *)
+  Hacl.EC.Curve25519.exp key pk sk;
+  let z = crypto_secretbox_detached c mac m mlen n key in
+  pop_frame();
+  z
 
 
-val crypto_box_open_easy:
+val crypto_box_open_detached:
   m:uint8_p ->
   c:uint8_p ->
   mac:uint8_p{length mac = crypto_box_MACBYTES} ->
@@ -61,3 +87,11 @@ val crypto_box_open_easy:
   Stack u32
     (requires (fun h -> live h c /\ live h m /\ live h n /\ live h pk /\ live h sk))
     (ensures  (fun h0 z h1 -> modifies_1 c h0 h1 /\ live h1 c))
+let crypto_box_open_detached m c mac mlen n pk sk =
+  push_frame();
+  let key = create (Hacl.Cast.uint8_to_sint8 0uy) 32ul in
+  (* Compute shared key *)
+  Hacl.EC.Curve25519.exp key pk sk;
+  let z = crypto_secretbox_open_detached m c mac mlen n key in
+  pop_frame();
+  z
