crypto_hst/Hacl.Constants.fst
@@ -13,11 +13,11 @@ type uint8_p = FStar.Buffer.buffer h8
 let crypto_box_NONCEBYTES     = 4
 let crypto_box_PUBLICKEYBYTES = 32
 let crypto_box_SECRETKEYBYTES = 32
-let crypto_box_MACBYTES       = 32
+let crypto_box_MACBYTES       = 16
 
 let crypto_secretbox_NONCEBYTES = 4
 let crypto_secretbox_KEYBYTES   = 32
-let crypto_secretbox_MACBYTES   = 32
+let crypto_secretbox_MACBYTES   = 16
 
 (* (\* Define hash algorithms *\) *)
 (* type hash_alg =  *)
