crypto_hst/Hacl.SecretBox.fst
@@ -3,7 +3,7 @@ module Hacl.SecretBox
 open FStar.Buffer
 open FStar.HST
 open Hacl.Constants
-
+open Hacl.Policies
 
 (* Module abbreviations *)
 module HS  = FStar.HyperStack
@@ -16,29 +16,6 @@ module U64 = FStar.UInt64
    disjointness clauses
 *)
 
-(* 
-   From libsodium documentation: c & m may overlap which allows for inplace encrypto
-   -> adapt implementation 
-   *)
-val crypto_secretbox_easy:
-  c:uint8_p ->
-  m:uint8_p ->
-  mlen:u64{let len = U64.v mlen in len <= length m /\ len + crypto_secretbox_MACBYTES <= length c}  ->
-  n:uint8_p{length n = crypto_secretbox_NONCEBYTES} ->
-  k:uint8_p{length k = crypto_secretbox_KEYBYTES} ->
-  Stack u32
-    (requires (fun h -> live h c /\ live h m /\ live h n /\ live h k))
-    (ensures  (fun h0 z h1 -> modifies_1 c h0 h1 /\ live h1 c))
-
-val crypto_secretbox_open_easy:
-  m:uint8_p ->
-  c:uint8_p ->
-  clen:u64{let len = U64.v clen in len = length m + crypto_secretbox_MACBYTES /\ len = length c}  ->
-  n:uint8_p{length n = crypto_secretbox_NONCEBYTES} ->
-  k:uint8_p{length k = crypto_secretbox_KEYBYTES} ->
-  Stack u32
-    (requires (fun h -> live h c /\ live h m /\ live h n /\ live h k))
-    (ensures  (fun h0 z h1 -> modifies_1 m h0 h1 /\ live h1 m))
 
 val crypto_secretbox_detached:
   c:uint8_p ->
@@ -50,14 +27,68 @@ val crypto_secretbox_detached:
   Stack u32
     (requires (fun h -> live h c /\ live h mac /\ live h m /\ live h n /\ live h k))
     (ensures  (fun h0 z h1 -> modifies_2 c mac h0 h1 /\ live h1 c /\ live h1 mac))
+let crypto_secretbox_detached c mac m mlen n k =
+  let mlen = Int.Cast.uint64_to_uint32 mlen in
+  Hacl.Symmetric.Chacha20.chacha20_encrypt c k (Hacl.Cast.uint32_to_sint32 1ul) n m mlen;
+  Hacl.Symmetric.Poly1305.poly1305_mac mac c mlen k;
+  0ul
+
 
 val crypto_secretbox_open_detached:
   m:uint8_p ->
   c:uint8_p ->
-  mac:uint8_p{length mac = crypto_secretbox_MACBYTES} ->
+  mac:uint8_p{length mac = crypto_secretbox_MACBYTES /\ declassifiable mac} ->
   clen:u64{let len = U64.v clen in len = length m /\ len = length c}  ->
   n:uint8_p{length n = crypto_secretbox_NONCEBYTES} ->
   k:uint8_p{length k = crypto_secretbox_KEYBYTES} ->
   Stack u32
     (requires (fun h -> live h m /\ live h c /\ live h mac /\ live h n /\ live h k))
     (ensures  (fun h0 z h1 -> modifies_1 m h0 h1 /\ live h1 m))
+let crypto_secretbox_open_detached m c mac clen n k =
+  push_frame();
+  let clen = Int.Cast.uint64_to_uint32 clen in
+  let tmp_mac = create (Hacl.Cast.uint8_to_sint8 0uy) 16ul in
+  Hacl.Symmetric.Poly1305.poly1305_mac tmp_mac c clen k;
+  assume (Hacl.Policies.declassifiable tmp_mac);
+  let verify = cmp_bytes mac tmp_mac 16ul in
+  if U8 (verify =^ 0uy) then (
+    Hacl.Symmetric.Chacha20.chacha20_encrypt m k (Hacl.Cast.uint32_to_sint32 1ul) n c clen;
+    pop_frame();
+    0x0ul
+  )
+  else (
+    pop_frame();
+    0xfffffffful
+  )
+
+
+val crypto_secretbox_easy:
+  c:uint8_p ->
+  m:uint8_p ->
+  mlen:u64{let len = U64.v mlen in len <= length m /\ len + crypto_secretbox_MACBYTES <= length c}  ->
+  n:uint8_p{length n = crypto_secretbox_NONCEBYTES} ->
+  k:uint8_p{length k = crypto_secretbox_KEYBYTES} ->
+  Stack u32
+    (requires (fun h -> live h c /\ live h m /\ live h n /\ live h k))
+    (ensures  (fun h0 z h1 -> modifies_1 c h0 h1 /\ live h1 c))
+let crypto_secretbox_easy c m mlen n k =
+  let mlen_ = FStar.Int.Cast.uint64_to_uint32 mlen in
+  let c = sub c 0ul mlen_ in
+  let mac = sub c mlen_ 16ul in
+  crypto_secretbox_detached c mac m mlen n k
+
+
+val crypto_secretbox_open_easy:
+  m:uint8_p ->
+  c:uint8_p ->
+  clen:u64{let len = U64.v clen in len = length m + crypto_secretbox_MACBYTES /\ len = length c}  ->
+  n:uint8_p{length n = crypto_secretbox_NONCEBYTES} ->
+  k:uint8_p{length k = crypto_secretbox_KEYBYTES} ->
+  Stack u32
+    (requires (fun h -> live h c /\ live h m /\ live h n /\ live h k))
+    (ensures  (fun h0 z h1 -> modifies_1 m h0 h1 /\ live h1 m))
+let crypto_secretbox_open_easy m c clen n k =
+  let clen_ = FStar.Int.Cast.uint64_to_uint32 clen in
+  let c = sub c 0ul clen_ in
+  let mac = sub c clen_ 16ul in
+  crypto_secretbox_open_detached m c mac clen n k
